

EXERCISE 1

EXAM 25/01/2024

(y_1, \dots, y_5) sample from $Y_i \sim \text{Pois}(e^{\beta_1})$ indep. $i = 1, \dots, 5$
 (y_6, \dots, y_{10}) sample from $Y_i \sim \text{Pois}(e^{\beta_1 + \beta_2})$ indep. $i = 6, \dots, 10$

- a) $Y_i \sim \text{Poisson}(\mu_i)$ $i = 1, \dots, 10$ indep.
 $\eta_i = \beta_1 + \beta_2 x_i$ with $x_i = \begin{cases} 0 & i = 1, \dots, 5 \\ 1 & i = 6, \dots, 10 \end{cases}$
 $\log \mu_i = \eta_i$

b) $p(y_i; \mu_i) = e^{-\mu_i} \mu_i^{y_i} \cdot \frac{1}{y_i!}$

$$p(y_1, \dots, y_{10} | \underline{\mu}) = \prod_{i=1}^{10} \left(e^{-\mu_i} \mu_i^{y_i} \frac{1}{y_i!} \right) \quad \text{with } \mu_i = e^{\tilde{x}_i^T \beta}$$

$$L(\underline{\beta}) \propto \prod_{i=1}^{10} e^{-\mu_i} \mu_i^{y_i} = \prod_{i=1}^{10} e^{-e^{\tilde{x}_i^T \beta}} e^{\tilde{x}_i^T \beta y_i}$$

$$\ell(\underline{\beta}) = \sum_{i=1}^{10} -e^{\tilde{x}_i^T \beta} + y_i \tilde{x}_i^T \beta$$

here, $\tilde{x}_i^T \beta = \beta_1 + \beta_2 x_i$ with x_i dummy variable, hence:

$$\begin{aligned} \ell(\beta_1, \beta_2) &= \sum_{i=1}^{10} \left\{ -e^{\beta_1 + \beta_2 x_i} + y_i (\beta_1 + \beta_2 x_i) \right\} \\ &= -\sum_{i=1}^{10} e^{\beta_1 + \beta_2 x_i} + \beta_1 \sum_{i=1}^{10} y_i + \beta_2 \sum_{i=1}^{10} x_i y_i \\ &= -\sum_{i=1}^5 e^{\beta_1} - \sum_{i=6}^{10} e^{\beta_1 + \beta_2} + \beta_1 \sum_{i=1}^{10} y_i + \beta_2 \sum_{i=6}^{10} y_i \\ &= -5e^{\beta_1} - 5e^{\beta_1 + \beta_2} + \beta_1 \sum_{i=1}^{10} y_i + \beta_2 \sum_{i=6}^{10} y_i \end{aligned}$$

$$\ell_{**}(\beta_1, \beta_2) = \begin{cases} \frac{\partial \ell(\underline{\beta})}{\partial \beta_1} = -5e^{\beta_1} - 5e^{\beta_1 + \beta_2} + \sum_{i=1}^{10} y_i \\ \frac{\partial \ell(\underline{\beta})}{\partial \beta_2} = -5e^{\beta_1 + \beta_2} + \sum_{i=6}^{10} y_i \end{cases} \quad \text{Score function}$$

$$\ell_{**}(\beta_1, \beta_2) = \begin{bmatrix} -5e^{\beta_1} - 5e^{\beta_1 + \beta_2} & -5e^{\beta_1 + \beta_2} \\ -5e^{\beta_1 + \beta_2} & -5e^{\beta_1 + \beta_2} \end{bmatrix} = -5 \begin{bmatrix} e^{\beta_1} + e^{\beta_1 + \beta_2} & e^{\beta_1 + \beta_2} \\ e^{\beta_1 + \beta_2} & e^{\beta_1 + \beta_2} \end{bmatrix}$$

observed info is $j(\underline{\beta}) = -\ell_{**}(\underline{\beta})$

The MLE can be found in closed-form by noticing that:

for sample 1 $\underline{y}_1 = (y_1, \dots, y_5)$ the expected value is $E[Y_i] = \mu_1 = e^{\beta_1}$
 for sample 2 $\underline{y}_2 = (y_6, \dots, y_{10})$ the expected value is $E[Y_i] = \mu_2 = e^{\beta_1 + \beta_2}$

The function from (β_1, β_2) to (μ_1, μ_2) is bijective (\Rightarrow invertible)

$$\begin{cases} \mu_1 = e^{\beta_1} \\ \mu_2 = e^{\beta_1 + \beta_2} \end{cases} \Leftrightarrow \begin{cases} \beta_1 = \log \mu_1 \\ \beta_1 + \beta_2 = \log \mu_2 \Rightarrow \beta_2 = \log \mu_2 - \log \mu_1 \end{cases}$$

I can obtain the MLE $(\hat{\mu}_1, \hat{\mu}_2)$ and obtain $(\hat{\beta}_1, \hat{\beta}_2) = f(\hat{\mu}_1, \hat{\mu}_2)$

The MLE of μ_1 and μ_2 are:

$$\begin{aligned} \hat{\mu}_1 &= \bar{y}_1 = \frac{1}{5} \sum_{i=1}^5 y_i \quad \text{sample mean of } \underline{y}_1 \\ \hat{\mu}_2 &= \bar{y}_2 = \frac{1}{5} \sum_{i=6}^{10} y_i \quad \text{sample mean of } \underline{y}_2 \end{aligned}$$

$$\Rightarrow \begin{cases} \hat{\beta}_1 = \log \hat{\mu}_1 \\ \hat{\beta}_2 = \log \hat{\mu}_2 - \log \hat{\mu}_1 \end{cases} \Rightarrow \begin{cases} \hat{\beta}_1 = \log \bar{y}_1 \\ \hat{\beta}_2 = \log \bar{y}_2 - \log \bar{y}_1 \end{cases}$$

Alternatively, one can solve the likelihood equations

$$\begin{cases} -5e^{\beta_1} - 5e^{\beta_1 + \beta_2} + \sum_{i=1}^{10} y_i = 0 \\ -5e^{\beta_1 + \beta_2} + \sum_{i=6}^{10} y_i = 0 \end{cases} \Rightarrow \begin{cases} 5e^{\beta_1 + \beta_2} = -5e^{\beta_1} + \sum_{i=1}^{10} y_i \\ 5e^{\beta_1 + \beta_2} = \sum_{i=6}^{10} y_i \end{cases}$$

$$\Rightarrow -5e^{\beta_1} + \sum_{i=1}^{10} y_i = \sum_{i=6}^{10} y_i$$

$$e^{\beta_1} = \frac{1}{5} \left(\sum_{i=1}^{10} y_i - \sum_{i=6}^{10} y_i \right) = \frac{1}{5} \sum_{i=1}^5 y_i = \bar{y}_1 \Rightarrow \hat{\beta}_1 = \log \bar{y}_1$$

From eq. 2: $5e^{\beta_1} e^{\beta_2} = \sum_{i=6}^{10} y_i \Rightarrow e^{\beta_2} = \frac{1}{5} \sum_{i=6}^{10} y_i e^{-\beta_1}$
 $\beta_2 = \log \bar{y}_2 - \beta_1 \Rightarrow \hat{\beta}_2 = \log \bar{y}_2 - \log \bar{y}_1$

c) $\begin{bmatrix} \hat{\beta}_1 \\ \hat{\beta}_2 \end{bmatrix} \sim N_2 \left(\begin{bmatrix} \beta_1 \\ \beta_2 \end{bmatrix}, j(\hat{\underline{\beta}})^{-1} \right)$

the marginal $\hat{\beta}_1 \sim N(\beta_1, [j(\hat{\underline{\beta}})^{-1}]_{(1,1)})$
 \hookrightarrow element in position (1,1)

d) we already noticed that

for sample 1 $E[Y_i] = \mu_1 = e^{\beta_1}$
 for sample 2 $E[Y_i] = \mu_2 = e^{\beta_1 + \beta_2}$

$$\frac{\mu_2}{\mu_1} = \frac{e^{\beta_1 + \beta_2}}{e^{\beta_1}} = e^{\beta_2} \Rightarrow \beta_2 = \log \frac{\mu_2}{\mu_1} = \log \frac{E[Y_i | \text{sample 2}]}{E[Y_i | \text{sample 1}]}$$

Hence β_2 represents the log of the ratio between the expected counts of the two samples.

Or, noting that $\mu_2 = e^{\beta_2} \cdot \mu_1$:

the expected counts of sample 2 are obtained by multiplying the expected counts of sample 1 by a coefficient e^{β_2} .

e) The saturated model is a model with n parameters μ_1, \dots, μ_n .

In this case, I have one parameter for each observation and the estimates are $\hat{\mu}_i^s = y_i \quad \forall i$

The loglikelihood for an individual observation is

$$\ell(\mu_i^s) = -\mu_i^s + y_i \log \mu_i^s$$

Hence the max of the loglikelihood is

$$\tilde{\ell}(\text{saturated}) = \sum_{i=1}^{10} \left\{ -\hat{\mu}_i^s + y_i \log \hat{\mu}_i^s \right\} = \sum_{i=1}^{10} \left\{ -y_i + y_i \log y_i \right\}$$